formal/AExp.thy
@@ -131,7 +131,8 @@ next
 qed
 
 lemma input2state_cons:
-  "x1 < length ia \<Longrightarrow>
+  "x1 > 0 \<Longrightarrow>
+   x1 < length ia \<Longrightarrow>
    input2state (a # ia) x1 = input2state ia (x1-1)"
   by (simp add: input2state_nth)
 
