formal/inference/Enable_Logging.thy
@@ -15,7 +15,7 @@ fun value2string :: "value \<Rightarrow> String.literal" where
   "value2string (value.Str s) = STR ''\"''+s+STR ''\"''"
 
 fun vname2string :: "vname \<Rightarrow> String.literal" where
-  "vname2string (I n) = STR ''i''+show_nat n" |
+  "vname2string (vname.I n) = STR ''i''+show_nat n" |
   "vname2string (R s) = STR ''r''+show_nat s"
 
 fun aexp2string :: "aexp \<Rightarrow> String.literal" where
